.dir-locals.el
@@ -1,4 +1,6 @@
-((coq-mode . ((eval . (let ((default-directory (locate-dominating-file
+((nil . ((eval . (setq default-directory (locate-dominating-file ; Always run make in the root directory
+					  buffer-file-name ".dir-locals.el")))))
+ (coq-mode . ((eval . (let ((default-directory (locate-dominating-file
 						buffer-file-name ".dir-locals.el")))
 			(make-local-variable 'coq-load-path)
 			(setq coq-load-path `((,(expand-file-name ".") "ADTSynthesis"))))))))
